Inversion lemmas done, and some work on t_thin

dev2020/dsubsup_cc/d2cc.v
@@ -125,17 +125,20 @@ Proof.
   - simpl. intros. rewrite IHG'. reflexivity.
 Qed.
 
-Lemma lookup_not_x : forall ty G G' x (T T' U : ty),
+Lemma lookup_change : forall ty G' G x (T U : ty), 
   lookup (G ~ T +~ G') x U ->
   x <> length G ->
+  forall T',
   lookup (G ~ T' +~ G') x U.
 Proof.
-  intros. destruct (x ?= length G) eqn:E.
-  - assert (x = length G). admit (*E*). contradiction.
-  - admit (* TODO: Case when x is in G *).
-  - admit (* TODO: Case when x is in G' *).
-Admitted.
-
+  induction G'.
+  - constructor. inversion H; subst. contradiction. assumption.
+  - simpl. inversion 1; subst.
+    + intros. replace (length (G ~ T +~ G')) with (length (G ~ T' +~ G')).
+      constructor. repeat rewrite length_elim_middle. reflexivity.
+    + constructor. eapply IHG'; eassumption.
+Qed.
+  
 
 Lemma split_nat : forall m n : nat, n <= m -> ((m - n) + n)%nat = m.
 Proof. lia. Qed.
@@ -374,7 +377,7 @@ Module CC.
     | tLam : expr -> expr -> expr
     | tApp : expr -> expr -> expr
     | TSig : expr -> expr -> expr
-    | tPair : expr -> expr -> expr -> expr
+    | tPair : expr -> expr -> expr -> expr -> expr
     | tFst : expr -> expr
     | tSnd : expr -> expr.
 
@@ -383,7 +386,7 @@ Module CC.
 
   Notation "\: T" := (tLam T) (at level 5) : cc_scope.
   Notation "t $" := (tApp t) (at level 4) : cc_scope.
-  Notation "t & u :[ T ]" := (tPair t u T) (at level 4) : cc_scope.
+  Notation "t & u :[ T ** U ]" := (tPair t u T U) (at level 4) : cc_scope.
   Coercion TSort : sort >-> expr.
   Coercion tVar : var >-> expr.
 
@@ -400,7 +403,8 @@ Module CC.
     | \:T t => \:(e{i :-> e'} T) (e{S i :-> e'} t)
     | t $ u => (e{i :-> e'} t) $ (e{i :-> e'} u)
     | TSig T U => TSig (e{i :-> e'} T) (e{S i :-> e'} U)
-    | t & u :[T] => (e{i :-> e'} t) & (e{i :-> e'} u) :[e{i :-> e'} T]
+    | t & u :[T ** U] => 
+        (e{i :-> e'} t) & (e{i :-> e'} u) :[e{i :-> e'} T ** e{i :-> e'} U]
     | tFst t => tFst (e{i :-> e'} t)
     | tSnd t => tSnd (e{i :-> e'} t)
     end
@@ -416,12 +420,31 @@ Module CC.
   Reserved Notation "G |-q e == u : T" (no associativity, at level 90,
                                           u at next level).
 
+  (* Closed expressions *)
+  Inductive closed (b f : nat) : expr -> Prop :=
+    | cl_sort : forall s : sort, closed b f s
+    | cl_varF : forall x, x < f -> closed b f `x
+    | cl_varB : forall i, i < f -> closed b f #i
+    | cl_all : forall T U, 
+        closed b f T -> closed (S b) f U -> closed b f (TAll T U)
+    | cl_lam : forall T e,
+        closed b f T -> closed (S b) f e -> closed b f (\:T e)
+    | cl_app : forall t u,
+        closed b f t -> closed b f u -> closed b f (t $ u)
+    | cl_sig : forall T U,
+        closed b f T -> closed (S b) f U -> closed b f (TSig T U)
+    | cl_pair : forall t u T U,
+        closed b f t -> closed b f u -> closed b f (TSig T U) ->
+        closed b f (t & u :[T ** U])
+    | cl_fst : forall t, closed b f t -> closed b f (tFst t)
+    | cl_snd : forall t, closed b f t -> closed b f (tSnd t).
+
   (* Full beta-pi reduction *)
   (* TODO: Do we need eta equality? *)
   Inductive reduce : expr -> expr -> Prop :=
     | r_beta : forall T e u, (\:T e) $ u ~~> e *^ u
-    | r_pi1 : forall e u T, tFst (e & u :[T]) ~~> e
-    | r_pi2 : forall e u T, tSnd (e & u :[T]) ~~> u
+    | r_pi1 : forall e u T U, tFst (e & u :[T ** U]) ~~> e
+    | r_pi2 : forall e u T U, tSnd (e & u :[T ** U]) ~~> u
     | r_all1 : forall T U T', T ~~> T' -> TAll T U ~~> TAll T' U
     | r_all2 : forall T U U', U ~~> U' -> TAll T U ~~> TAll T U'
     | r_lam1 : forall T e T', T ~~> T' -> \:T e ~~> \:T' e
@@ -433,26 +456,31 @@ Module CC.
     (* The lecture notes linked above don't mention adding these 
        substructural rules for pairs, but I think they're required, else
        we can't reduce inside tuples. *)
-    | r_pair1 : forall t u T t', t ~~> t' -> (t & u :[T]) ~~> (t' & u :[T])
-    | r_pair2 : forall t u T u', u ~~> u' -> (t & u :[T]) ~~> (t & u' :[T])
-    | r_pair3 : forall t u T T', T ~~> T' -> (t & u :[T]) ~~> (t & u :[T'])
+    | r_pair1 : forall t u T U t', 
+        t ~~> t' -> (t & u :[T ** U]) ~~> (t' & u :[T ** U])
+    | r_pair2 : forall t u T U u', 
+        u ~~> u' -> (t & u :[T ** U]) ~~> (t & u' :[T ** U])
+    | r_pair3 : forall t u T T' U, 
+        T ~~> T' -> (t & u :[T ** U]) ~~> (t & u :[T' ** U])
+    | r_pair4 : forall t u T U U',
+        U ~~> U' -> (t & u :[T ** U]) ~~> (t & u :[T ** U'])
     | r_fst : forall t t', t ~~> t' -> tFst t ~~> tFst t'
     | r_snd : forall t t', t ~~> t' -> tSnd t ~~> tSnd t'
-    where "e ~~> u" := (reduce e u) : cc_scope.
-
-  (* Beta-pi equality *)
-  Inductive equals : expr -> expr -> Prop :=
-    | e_red : forall e u, e ~~> u -> e == u
-    | e_refl : forall e, e == e
-    | e_sym : forall e u, e == u -> u == e
-    | e_trans : forall e u t, e == u -> u == t -> e == t
-    where "e == u" := (equals e u) : cc_scope.
-
-  (* Context formation *)
-  Inductive wfCx : cx -> Prop :=
-    | wf_nil : nil |-cc
-
-    | wf_cons: forall G T s,
+     where "e ~~> u" := (reduce e u) : cc_scope.
+ 
+   (* Beta-pi equality *)
+   Inductive equals : expr -> expr -> Prop :=
+     | e_red : forall e u, e ~~> u -> e == u
+     | e_refl : forall e, e == e
+     | e_sym : forall e u, e == u -> u == e
+     | e_trans : forall e u t, e == u -> u == t -> e == t
+     where "e == u" := (equals e u) : cc_scope.
+ 
+   (* Context formation *)
+   Inductive wfCx : cx -> Prop :=
+     | wf_nil : nil |-cc
+ 
+     | wf_cons: forall G T s,
         G |-cc ->
         G |-e T : TSort s ->
         G ~ T |-cc
@@ -469,11 +497,14 @@ Module CC.
         G |-e `x : T
 
     | t_all : forall G T U sT sU,
+        closed 1 (length G) U ->
         G |-e T : TSort sT ->
         G ~ T |-e U *^ varF (length G) : TSort sU ->
         G |-e TAll T U : TSort sU
 
     | t_lam : forall G T U e s,
+        closed 0 (length G) (TAll T U) ->
+        closed 1 (length G) e ->
         G |-e T : TSort s ->
         G ~ T |-e e *^ varF (length G) : U *^ varF (length G) ->
         G |-e \:T e : TAll T U
@@ -484,6 +515,7 @@ Module CC.
         G |-e t $ u : U *^ u
 
     | t_sig : forall G T U sT sU,
+        closed 1 (length G) U ->
         G |-e T : TSort sT ->
         G ~ T |-e U *^ varF (length G) : TSort sU ->
         G |-e TSig T U : TSort sU
@@ -492,7 +524,7 @@ Module CC.
         G |-e TSig T U : TSort s ->
         G |-e t : T ->
         G |-e u : U *^ t ->
-        G |-e t & u :[TSig T U] : TSig T U
+        G |-e t & u :[T ** U] : TSig T U
 
     | t_fst : forall G T U e,
         G |-e e : TSig T U ->
@@ -515,6 +547,55 @@ Module CC.
   
   Hint Constructors wfCx hasType equals : Core.
 
+  (* Size of an expression is the number of non-leaf nodes in the AST. *)
+  Fixpoint esize_flat (e : expr) : nat :=
+    match e with
+    | TSort _ | tVar _ => 0
+    | TAll T U | \:T U | T $ U | TSig T U => S (esize_flat T + esize_flat U)
+    | t & u :[T ** U] => 
+        S (esize_flat t + esize_flat u + esize_flat T + esize_flat U)
+    | tFst t | tSnd t => S (esize_flat t)
+    end.
+
+  (* Opening an expression with a free variable does not change its size. *)
+  Lemma esize_open : forall e x i, esize_flat e = esize_flat (e{i :-> `x} e).
+  Proof.
+    induction e; simpl; intros;
+    try (rewrite <- IHe1; rewrite <- IHe2); 
+    try (rewrite <- IHe3; rewrite <- IHe4);
+    try rewrite <- IHe;
+    try (destruct v; try destruct (i =? b)); reflexivity.
+  Qed.
+
+  (* A well-founded relation *)
+  Inductive R : expr -> expr -> Prop :=
+    | lt_all1 : forall T U, R T (TAll T U)
+    | lt_all2 : forall T U (G : list expr), R (U *^ ` (length G)) (TAll T U)
+    | lt_lam1 : forall T e, R T (\:T e)
+    | lt_lam2 : forall T e (G : list expr), R (e *^ ` (length G)) (\:T e)
+    | lt_app1 : forall t u, R t (t $ u)
+    | lt_app2 : forall t u, R u (t $ u)
+    | lt_sig1 : forall T U, R T (TSig T U)
+    | lt_sig2 : forall T U (G : list expr), R (U *^ ` (length G)) (TSig T U)
+    | lt_pair1 : forall t u T U, R t (t & u :[T ** U])
+    | lt_pair2 : forall t u T U, R u (t & u :[T ** U])
+    | lt_pairT : forall t u T U, R T (t & u :[T ** U])
+    | lt_pairU : forall t u T U, R U (t & u :[T ** U])
+    | lt_fst : forall t, R t (tFst t)
+    | lt_snd : forall t, R t (tSnd t).
+
+  (* Proof that R is well-founded. *)
+  Lemma wfR' : forall n e, esize_flat e <= n -> Acc R e.
+  Proof.
+    induction n; destruct e; constructor; inversion 1; subst; simpl in *;
+    try (apply IHn; try rewrite <- esize_open); lia.
+  Qed.
+
+  Lemma wfR : well_founded R.
+  Proof.
+    red. intros e. eapply wfR'. auto.
+  Qed.
+
   (* Substitution *)
   Reserved Notation "e[ x :-> u ]" (at level 50).
   Fixpoint subst (x : fVar) (u e : expr) : expr :=
@@ -525,7 +606,8 @@ Module CC.
     | \:T t => \:(e[x :-> u] T) (e[x:-> u] t)
     | t $ t' => (e[x :-> u] t) $ (e[x :-> u] t')
     | TSig T U => TSig (e[x :-> u] T) (e[x :-> u] U)
-    | t & t' :[T] => (e[x :-> u] t) & (e[x :-> u] t') :[e[x :-> u] T]
+    | t & t' :[T ** U] => 
+        (e[x :-> u] t) & (e[x :-> u] t') :[e[x :-> u] T ** e[x :-> u] U]
     | tFst t => tFst (e[x :-> u] t) 
     | tSnd t => tSnd (e[x :-> u] t)
     end
@@ -541,7 +623,7 @@ Module CC.
     | \:T t => \:(k +> T) (k +> t)
     | t $ u => (k +> t) $ (k +> u)
     | TSig T U => TSig (k +> T) (k +> U)
-    | t & u :[T] => (k +> t) & (k +> u) :[k +> T]
+    | t & u :[T ** U] => (k +> t) & (k +> u) :[k +> T ** k +> U]
     | tFst t => tFst (k +> t)
     | tSnd t => tSnd (k +> t)
     end
@@ -557,40 +639,147 @@ Module CC.
     | \:T t => \:(k -< T) (k -< t)
     | t $ u => (k -< t) $ (k -< u)
     | TSig T U => TSig (k -< T) (k -< U)
-    | t & u :[T] => (k -< t) & (k -< u) :[k -< T]
+    | t & u :[T ** U] => (k -< t) & (k -< u) :[k -< T ** k -< U]
     | tFst t => tFst (k -< t)
     | tSnd t => tSnd (k -< t)
     end
     where "k -<" := (unsplice k) : cc_scope.
 
-  (* Renaming *)
-  Reserved Notation "x <~> y" (at level 45, right associativity).
-  Fixpoint rename (x y : fVar) (e : expr) : expr :=
-    match e with
-    | tVar `w => if x =? w then `y else if y =? w then `x else `w
-    | TSort _ | tVar #_ => e
-    | TAll T U => TAll ((x <~> y) T) ((x <~> y) U)
-    | \:T t => \:((x <~> y) T) ((x <~> y) t)
-    | t $ u => ((x <~> y) t) $ ((x <~> y) u)
-    | TSig T U => TSig ((x <~> y) T) ((x <~> y) U)
-    | t & u :[T] => ((x <~> y) t) & ((x <~> y) u) :[(x <~> y) T]
-    | tFst t => tFst ((x <~> y) t)
-    | tSnd t => tSnd ((x <~> y) t)
-    end
-    where "x <~> y" := (rename x y) : cc_scope.
-
-  (* Unsplicing is the inverse of splicing. *)
-  Lemma splice_unsplice : forall e k, k -< (k +> e) = e.
+  (**************************************************************************
+   * Rules for Equality *)
+  Lemma e_sig1 : forall T1 T2, 
+    T1 == T2 ->
+    forall U, TSig T1 U == TSig T2 U.
   Proof.
-    induction e; simpl; intros; try (rewrite IHe1; rewrite IHe2); 
-    try rewrite IHe3; try rewrite IHe; try reflexivity.
-    - destruct v. reflexivity. destruct (k <=? f) eqn:E.
-      + simpl. replace (k <=? S f) with true (* since k <= f *).
-        assert (f - 0 = f). lia. rewrite H. reflexivity. 
-        assert (k <= f). apply Nat.leb_le. assumption.
-        assert (k <= S f). lia.
-        apply Nat.leb_le in H0. symmetry. assumption.
-      + simpl. rewrite E. reflexivity.
+    induction 1; intros.
+    - eapply e_trans. apply e_red. apply r_sig1. eassumption. apply e_refl.
+    - apply e_refl.
+    - apply e_sym. apply IHequals.
+    - eapply e_trans; auto.
+  Qed.
+
+  (**************************************************************************
+   * Inversion Lemmas *)
+  Lemma hasType_inversion_sort : forall (s : sort) G T,
+    G |-e s : T -> s = prop /\ (T == type).
+  Proof.
+    intros. remember (TSort s0) as e. induction H; subst; try discriminate.
+    - inversion Heqe. split. reflexivity. apply e_refl.
+    - assert (TSort s0 = s0) by reflexivity. apply IHhasType in H1. split.
+      apply H1. eapply e_trans. apply e_sym. eassumption. apply H1.
+  Qed.
+  
+  Lemma hasType_inversion_varB : forall i G T, ~ (G |-e #i : T).
+  Proof.
+    unfold not. intros. remember (tVar #i) as v. 
+    induction H; try discriminate.
+    apply IHhasType. assumption.
+  Qed.
+
+  Lemma hasType_inversion_varF : forall x G T,
+    G |-e `x : T -> lookup G x T \/ exists U, lookup G x U /\ (U == T).
+  Proof.
+    intros x. remember (tVar `x) as v. induction 1; try discriminate; subst.
+    - inversion Heqv. subst. left. assumption.
+    - right. assert (tVar `x = `x). reflexivity. apply IHhasType in H1.
+      destruct H1.
+      + exists T. split; assumption.
+      + do 2 destruct H1. exists x0. split. assumption. eapply e_trans.
+        eassumption. assumption.
+  Qed.
+
+  Lemma hasType_inversion_all : forall T U G V,
+    G |-e TAll T U : V -> 
+    closed 1 (length G) U /\
+    (exists sT : sort, G |-e T : sT) /\
+    (exists sU : sort, (V == sU) /\ (G ~ T |-e U *^ ` (length G) : sU)).
+  Proof.
+    intros. remember (TAll T U) as e. induction H; subst; try discriminate.
+    - inversion Heqe. subst. split. assumption. split. exists sT. assumption. 
+      exists sU. split. apply e_refl. assumption.
+    - intuition. destruct H1. destruct H4. destruct H3. exists x0. split.
+      eapply e_trans. apply e_sym. eassumption. assumption. assumption.
+  Qed.
+
+  Lemma hasType_inversion_lam : forall T e G V,
+    G |-e \:T e : V ->
+    closed 1 (length G) e /\
+    (exists sT : sort, G |-e T : sT) /\
+    exists U, (V == TAll T U) /\
+    (closed 0 (length G) (TAll T U)) /\
+    (G ~ T |-e e *^ ` (length G) : U *^ ` (length G)).
+  Proof.
+    intros. remember (\:T e) as t. induction H; subst; try discriminate.
+    - inversion Heqt. subst. split. assumption. split. exists s0. assumption.
+      exists U. split. apply e_refl. split; assumption.
+    - intuition. destruct H1. destruct H4. destruct H3. destruct H4. 
+      exists x0. split. eapply e_trans. apply e_sym. eassumption. assumption. 
+      split; assumption.
+  Qed.
+
+  Lemma hasType_inversion_app : forall e u G V,
+    G |-e e $ u : V ->
+    exists U, (V == U *^ u) /\ 
+    exists T, (G |-e e : TAll T U) /\ (G |-e u : T).
+  Proof.
+    intros. remember (e $ u) as t. induction H; subst; try discriminate.
+    - inversion Heqt. subst. exists U. split. apply e_refl. exists T.
+      split; assumption.
+    - assert (e $ u = e $ u) by reflexivity. apply IHhasType in H1.
+      do 2 destruct H1. do 2 destruct H2. exists x. split.
+      + eapply e_trans. apply e_sym. eassumption. assumption.
+      + exists x0. split; assumption.
+  Qed.
+
+  Lemma hasType_inversion_sig : forall T U G V,
+    G |-e TSig T U : V -> 
+    closed 1 (length G) U /\
+    (exists sT : sort, G |-e T : sT) /\
+    (exists sU : sort, (V == sU) /\ (G ~ T |-e U *^ ` (length G) : sU)).
+  Proof.
+    intros. remember (TSig T U) as e. induction H; subst; try discriminate.
+    - inversion Heqe. subst. split. assumption. split. exists sT. assumption.
+      exists sU. split. apply e_refl. assumption.
+    - intuition. destruct H1. destruct H4. destruct H3. exists x0. split. 
+      eapply e_trans. apply e_sym. eassumption. assumption. assumption.
+  Qed.
+
+  Lemma hasType_inversion_pair : forall t u T G U V,
+    G |-e (t & u :[T ** U]) : V ->
+    (V == TSig T U) /\
+    (G |-e t : T) /\
+    (G |-e u : U *^ t) /\
+    exists s : sort, G |-e TSig T U : s.
+  Proof.
+    intros. remember (t & u :[T ** U]) as e. 
+    induction H; subst; try discriminate.
+    - inversion Heqe. subst. split. apply e_refl. split. assumption.
+      split. assumption. exists s0. assumption.
+    - intuition. eapply e_trans. apply e_sym. eassumption. assumption.
+  Qed.
+
+  Lemma hasType_inversion_fst : forall t G T,
+    G |-e tFst t : T ->
+    exists U, G |-e t : TSig T U.
+  Proof.
+    intros. remember (tFst t) as e. induction H; subst; try discriminate.
+    - inversion Heqe. subst. exists U. assumption.
+    - assert (tFst t = tFst t) by reflexivity. apply IHhasType in H1.
+      destruct H1. exists x. eapply t_conv. eassumption. apply e_sig1.
+      assumption.
+  Qed.
+
+  Lemma hasType_inversion_snd : forall t G V,
+    G |-e tSnd t : V ->
+    exists U, (V == U *^ tFst t) /\
+    exists T, G |-e t : TSig T U.
+  Proof.
+    intros. remember (tSnd t) as e. induction H; subst; try discriminate.
+    - inversion Heqe. subst. exists U. split. apply e_refl. exists T.
+      assumption.
+    - assert (tSnd t = tSnd t) by reflexivity. apply IHhasType in H1.
+      do 2 destruct H1. destruct H2. exists x. split. eapply e_trans.
+      apply e_sym. eassumption. assumption. exists x0. assumption.
   Qed.
 
   (* Splicing distributes on opening. *)
@@ -598,7 +787,7 @@ Module CC.
     k +> (e{i :-> t} e) = e{i :-> k +> t} (k +> e).
   Proof.
     induction e; simpl; intros; 
-    try (rewrite IHe1; rewrite IHe2; try rewrite IHe3); 
+    try (rewrite IHe1; rewrite IHe2; try (rewrite IHe3; rewrite IHe4)); 
     try rewrite IHe;
     try reflexivity.
     - destruct v; simpl. 
@@ -606,269 +795,165 @@ Module CC.
       + reflexivity.
   Qed.
 
-  (* Renaming distributes on opening. *)
-  Lemma rename_open : forall e t x y i,
-    (x <~> y) (e{i :-> t} e) = e{i :-> (x <~> y) t} ((x <~> y) e).
+  (* Splicing at position f does not mutate an expression closed under f free
+     variables. *)
+  Lemma splice_closed : forall f e b, closed b f e -> f +> e = e.
   Proof.
-    induction e; simpl; intros;
-    try (rewrite IHe1; rewrite IHe2; try rewrite IHe3);
-    try rewrite IHe;
-    try reflexivity.
-    - destruct v; simpl.
-      + destruct (i =? b); reflexivity.
-      + destruct (x =? f), (y =? f); reflexivity.
+    induction 1; simpl; 
+    try (rewrite IHclosed1; rewrite IHclosed2);
+    try rewrite IHclosed.
+    2: destruct (f <=? x) eqn:E. 
+    2: apply Nat.leb_le in E; try lia.
+    1-10: try reflexivity.
+    inversion IHclosed3. subst. repeat rewrite H3. repeat rewrite H4. 
+    reflexivity.
   Qed.
 
-  (* Valid renamings *)
-  (* !!! *)
-  Lemma t_ren : forall G e T,
-    G |-e e : T ->
-    forall G' G1 T1 G2 T2 G3 r,
-    G = G1 ~ T1 +~ G2 ~ T2 +~ G3 ->
-    r = length G1 <~> length (G1 ~ T1 +~ G2) ->
-    G' = map r (G1 ~ T2 +~ G2 ~ T1 +~ G3) ->
-    G' |-cc ->
-    G' |-e r e : r T.
-  Proof.
-    induction 1; intros G' G1 T1 G2 T2 G3 r Geq req G'eq H'.
-    - rewrite req. constructor. assumption.
-    - rewrite req. simpl. destruct (length G1 =? x) eqn:E.
-      + constructor. assumption. rewrite G'eq. rewrite <- req. 
-        apply lookup_map. 
-        assert (length (G1 ~ T1 +~ G2) = length (G1 ~ T2 +~ G2)).
-        { repeat rewrite length_elim_middle. reflexivity. }
-        rewrite H1. simpl. 
-        assert (length G1 = x). { apply beq_nat_true. assumption. }
-        assert (T1 = T).
-        { eapply lookup_drop_r. rewrite Geq in H0. rewrite <- H2 in H0.
-          rewrite app_assoc in H0. eassumption. }
-        rewrite H3. apply lookup_append_r. constructor.
-      + destruct (length (G1 ~ T1 +~ G2) =? x) eqn:E'.
-        * constructor. assumption. rewrite G'eq. rewrite <- req.
-          apply lookup_map. 
-          assert (length (G1 ~ T1 +~ G2) = x). 
-          { apply beq_nat_true. assumption. }
-          assert (T2 = T).
-          { eapply lookup_drop_r. rewrite Geq in H0. 
-            rewrite <- app_comm_cons in H0. rewrite <- H1 in H0.
-          eassumption. }
-          rewrite <- H2. rewrite app_assoc. apply lookup_append_r. constructor.
-        * admit (* TODO: Use lookup_not_x *).
-    - rewrite req. simpl. rewrite <- req.
-      assert (G' |-e r T : sT).
-      { replace (TSort sT) with (r sT). eapply IHhasType1; eassumption.
-        rewrite req. reflexivity. }
-      econstructor. 
-      + eassumption. 
-      + replace (tVar (` (length G'))) with (r (` (length G))).
-        rewrite req. rewrite <- rename_open. 
-        replace (TSort sU) with (r sU). rewrite <- req.
-        eapply IHhasType2 with (G1 := G1) (G2 := G2) (G3 := G3 ~ T).
-        rewrite Geq. reflexivity. assumption. rewrite G'eq. reflexivity.
-        econstructor; eassumption. rewrite req. reflexivity. rewrite req.
-        admit (* length G not in {length G1, length G1 ~ T1 +~ G2} *).
-    - admit (* TODO: Similar to TAll case *).
-    - admit (* TODO *).
-    - admit (* TODO: Similar to TAll case *).
-    - admit (* TODO *).
-    - admit (* TODO *).
-    - admit (* TODO *).
-    - admit (* TODO *).
-  Admitted.
+  (* Splicing a sort does not change the sort. *)
+  Lemma splice_sort : forall s k, TSort s = k +> s.
+  Proof. reflexivity. Qed.
 
-  (* Any typing judgment under context G is valid under context G ~ T. *)
-  (* !!! *)
-  Lemma t_weaken : forall G e T,
-    G |-e e : T ->
-    forall U s, 
-    G |-e U : TSort s ->
-    G ~ U |-e e : T. 
-  Proof.
-    induction 1.
-    - constructor. econstructor; eassumption.
-    - constructor. econstructor; eassumption. constructor. assumption.
-    - econstructor.
-      + eapply IHhasType1. eassumption.
-      + remember (length G <~> length (G ~ U)) as r.
-        assert (r U = U).
-        { admit (* 
-              U is the body of the TAll, which is well formed under G.
-              Thus, it is not locally closed, but it does not contain
-              any free variables that are not in G.
-          *). }
-        assert (U *^ ` (length (G ~ U0)) = r (U *^ ` (length G))).
-        { rewrite Heqr. rewrite rename_open. simpl. rewrite <- beq_nat_refl.
-          simpl in Heqr. rewrite <- Heqr. rewrite H2. reflexivity. }
-        rewrite H3. 
-        replace (TSort sU) with (r sU).
-        apply t_ren with (G := G ~ T ~ U0) (G' := G ~ U0 ~ T)
-          (G1 := G) (T1 := T) (G2 := nil) (T2 := U0) (G3 := nil).
-        eapply IHhasType2.
-  Abort (* 
-      We're stuck trying to prove G ~ T |-e U0 : s0. We have G |-e U0 : s0,
-      but no suitable IH. We likely cannot use Fixpoint to give us more 
-      power, because we use renaming to prove that the codomain of TAll is
-      well-formed. However, this looks like a potential candidate for well-
-      founded recursion -- renaming doesn't grow the term. 
-  *).
-        
-
-  (* Any pretype in a context is a type. *)
-  Theorem wfCx_lookup : forall G,
-    G |-cc ->
-    forall T, In T G ->
-    exists s : sort, G |-e T : s.
-  Admitted.
-
-  Hint Resolve wfCx_lookup : core.
-
-  Lemma hasType_splice : forall G G' e T,
-    G' +~ G |-e e : T ->
-    forall U,
-    G' ~ U +~ map (length G' +>) G |-cc ->
-    G' ~ U +~ map (length G' +>) G |-e (length G' +> e) : (length G' +> T).
-  Proof.
-    (* Attempted induction on 1, nonsense IH2 in TAll case *)
-    intros ? ? ? ? ?. remember (G' +~ G) as G'G. induction H; subst.
-    - constructor. assumption.
-    - simpl. destruct (length G' <=? x) eqn:E.
-      + constructor. assumption. 
-        admit (* 
-            1. S x >= length (G' ~ U) -> S x = length (G' ~ U) + x' for some x'
-               TODO: Define split_nat.
-            2. Goal: lookup (map (length G' +>) G) x' (length G' +> T)
-               TODO: Prove that lookup (T +~ G) (S x) U -> lookup G x U
-            3. Goal: lookup G x' T
-               TODO: Prove lookup_map
-            H0: lookup G x' T
-        *).
-      + constructor. assumption.
-        admit (*
-            Goal: lookup (map (length G' +>) G' ~ U +~ map (length G' +>) G)
-                         x (length G' +> T)
-            Since x < length G',
-            Goal: lookup (map (length G' +>) G') x (length G' +> T)
-            Goal: lookup G' x T
-            H0: lookup G' x T
-        *).
-    - Abort (* That second induction hypothesis is nonsense. *).
-  (* forall n, esize_flat e <= n, lemma <<- guard the proof*)
-  Fixpoint hasType_splice G G' e T (H : G +~ G' |-e e : T)
-      : forall U, 
-        G ~ U +~ map (length G +>) G' |-cc -> 
-        G ~ U +~ map (length G +>) G' |-e length G +> e : length G +> T.
-  Proof.
-    remember (G +~ G') as GG'. 
-    assert (forall k (s : sort), TSort s = k +> s). reflexivity.
-    destruct H; subst.
-    - constructor. assumption.
-    - constructor. assumption. admit (* lookup_splice *).
-    - simpl. econstructor; erewrite H0. 
-      + apply hasType_splice; eassumption.
-      + (* Rewrite the expression to the form (length G +> (U *^ `x)) *)
-        rewrite length_elim_middle. 
-        assert (tVar (varF (S (length (G +~ map (length G +>) G')))) =
-                  length G +> (varF (length (G +~ map (length G +>) G')))).
-        { simpl. admit (* length G <= length (G +~ map (length G +>) G')*). }
-        rewrite H3. rewrite <- splice_open. 
-        (* Rewrite the context to the form (G1 ~ T +~ G2) *)
-        replace ((G ~ U0 +~ map (length G +>) G') ~ length G +> T) with
-          (G ~ U0 +~ map (length G +>) (G' ~ T)).
-        apply hasType_splice.
-        replace (G +~ G' ~ T) with ((G +~ G') ~ T). 
-        replace (length (G +~ map (length G +>) G')) with (length (G +~ G')).
-        assumption. admit (* map preserves length *). 
-        admit (* cons and append commute *). simpl. econstructor. assumption.
-        erewrite H0. apply hasType_splice. eassumption. assumption.
-        reflexivity.
-    - admit (* TODO: Should be same as TAll case *).
-    - admit (* TODO *).
-    - admit (* TODO: Should be same as TAll and tLam cases *).
-    - admit (* TODO *).
-    - admit (* TODO *).
-    - admit (* TODO *).
-  Abort (* I strongly suspect this proof will be rejected because Coq's 
-    primitive recursion scheme won't be able to tell that this definition is
-    indeed well-founded. I'd have to use well-founded recursion. But I'm not
-    clear what the well-founded relation should be here -- we have to prove
-    that U *^ (length G) < TAll T U. I suppose a relation which says that
-    opening U with a variable makes it less than TAll T U would work.
-  *).
-
-  (* This time, I'mma try using the Fix combinator. *)
-  Reserved Notation "e e<= u" (at level 90, no associativity).
-  Inductive expr_lt : expr -> expr -> Prop :=
-    | lt_sort : forall T s, TSort s e<= T
-    | lt_var : forall T x, tVar x e<= T
-    | lt_all1 : forall T U, T e<= TAll T U
-    | lt_all2 : forall T U, U e<= TAll T U
-    | lt_lam1 : forall T e, T e<= \:T e
-    | lt_lam2 : forall T e, e e<= \:T e
-    | lt_app1 : forall e u, e e<= e $ u
-    | lt_app2 : forall e u, u e<= e $ u
-    | lt_sig1 : forall T U, T e<= TSig T U
-    | lt_sig2 : forall T U, U e<= TSig T U
-    | lt_pair1 : forall t u T, t e<= (t & u :[T])
-    | lt_pair2 : forall t u T, u e<= (t & u :[T])
-    | lt_pair3 : forall t u T, T e<= (t & u :[T])
-    | lt_fst : forall t, t e<= tFst t
-    | lt_snd : forall t, t e<= tSnd t
-    | lt_open : forall e u i x, e e<= u -> e{i :-> tVar x} e e<= u
-    where "e e<= u" := (expr_lt e u) : cc_scope.
-
-  (* A more intuitive measure *)
-  Fixpoint esize_flat (e : expr) : nat :=
-    match e with
-    | TSort _ | tVar _ => 0
-    | TAll T U | \:T U | T $ U | TSig T U => S (esize_flat T + esize_flat U)
-    | t & u :[T] => S (esize_flat t + esize_flat u + esize_flat T)
-    | tFst t | tSnd t => S (esize_flat t)
-    end.
-
-  (* Opening with a variable preserves size *)
-  Lemma open_var_size : forall e x i,
-    esize_flat e = esize_flat (e{i :-> tVar x} e).
-  Proof.
-    induction e; intros; simpl; eauto.
-    destruct v; try destruct (i =? b); auto.
-  Qed.
-
-  Lemma wf'_expr_lt : forall n e, esize_flat e <= n -> Acc expr_lt e.
-  Proof.
-    induction n.
-    - destruct e; intros. constructor; intros; simpl in *; inversion H0;
-      subst; try lia. Print Acc. constructor.  admit (* TODO:% How do I proceed? :P *).
-  Admitted.
-
-  Theorem wf_expr_lt : well_founded expr_lt. Admitted.
-
-  Print Fix.
-  (*
-  Definition hasType_splice {G G' e T} 
-    (H1 : G' +~ G |-e e : T)
-    {U} (H2 : G' ~ U +~ map (length G' +>) G |-cc) :
-    G' ~ U +~ map (length G' +>) G |-e (length G' +> e) : (length G' +> T).
-  refine (
-  Fix wf_expr_lt 
-  (fun _ => 
-    G' ~ U +~ map (length G' +>) G |-e (length G' +> e) : (length G' +> T))
-  (fun ()))
-   *)
-
-  Lemma hasType_splice : forall G G' e T,
-    G' +~ G |-e e : T ->
-    forall U,
-    G' ~ U +~ map (length G' +>) G |-cc ->
-    G' ~ U +~ map (length G' +>) G |-e (length G' +> e) : (length G' +> T).
-  Proof. admit. Admitted.
-
-  (* If a term is well-typed under precontext G, then G is a context. *)
+  (* If an expression is well-typed under G, then G is a context. *)
   Theorem hasType_wfCx : forall G e T, G |-e e : T -> G |-cc.
   Proof.
     induction 1; try assumption.
   Qed.
 
   Hint Resolve hasType_wfCx : core.
+
+  (* Any pretype in a context is a type. *)
+  Theorem wfCx_lookup : forall G,
+    G |-cc ->
+    forall T, In T G ->
+    exists s : sort, G |-e T : s
+
+  (* Splicing preserves well-typedness. *)
+  with t_thin : forall e G G' T,
+    G +~ G' |-e e : T ->
+    forall U, G ~ U +~ map (length G +>) G' |-cc ->
+    G ~ U +~ map (length G +>) G' |-e length G +> e : length G +> T
+
+  (* Splicing preserves beta-pi equivalence. *)
+  with eq_splice : forall e u,
+    e == u ->
+    forall k, k +> e == k +> u
+
+  (* Splicing preserves lookups on context. *)
+  with lookup_splice : forall G' G,
+    G +~ G' |-cc ->
+    forall x T, lookup (G +~ G') x T ->
+    forall U, G ~ U +~ map (length G +>) G' |-cc ->
+    lookup (G ~ U +~ map (length G +>) G') 
+      (if length G <=? x then S x else x) (length G +> T)
+
+  (* Weakening rule *)
+  with t_weak : forall G e T,
+    G |-e e : T ->
+    forall U, G ~ U |-cc ->
+    G ~ U |-e e : T.
+  Proof.
+    * induction 1; inversion 1; subst. 
+      - exists s0. apply t_weak. assumption. econstructor; eassumption. 
+      - apply IHwfCx in H2 as H3. destruct H3. exists x. apply t_weak. 
+        assumption. econstructor; eassumption.
+    
+    * induction e using (well_founded_induction wfR); intros; 
+      apply hasType_wfCx in H0 as wfGG'; destruct e.
+      - simpl. apply hasType_inversion_sort in H0. destruct H0.
+        rewrite H0. econstructor. constructor. assumption.
+        replace (TSort type) with (length G +> type). apply eq_splice. 
+        apply e_sym. assumption. reflexivity.
+      - destruct v.
+        + apply hasType_inversion_varB in H0. contradiction.
+        + apply hasType_inversion_varF in H0. destruct H0.
+          -- constructor. assumption. apply lookup_splice. assumption.
+             assumption. assumption.
+          -- destruct H0. destruct H0. remember (length G +> T) as T'.
+             eapply t_conv. constructor. assumption. apply lookup_splice.
+             assumption. eassumption. assumption. subst. apply eq_splice.
+             assumption.
+      - simpl. apply hasType_inversion_all in H0. destruct H0.
+        do 2 destruct H2. do 2 destruct H3. remember (length G +> T) as T'. 
+        eapply t_conv. econstructor. admit (* Some lemma on closed splicing *).
+        erewrite splice_sort. apply H. constructor. eassumption. assumption.
+        assert (tVar ` (length (G ~ U +~ map (length G +>) G')) = 
+                length G +> ` (length (G +~ G'))).
+        { rewrite length_elim_middle. simpl. 
+          replace (length G <=? length (G +~ G')) with true. 
+          repeat rewrite app_length. rewrite map_length. reflexivity. 
+          symmetry. rewrite Nat.leb_le. rewrite app_length. lia. }
+        rewrite H4. rewrite <- splice_open. 
+        assert ((G ~ U +~ map (length G +>) G') ~ length G +> e1 = 
+                G ~ U +~ map (length G +>) (G' ~ e1)) by reflexivity.
+        rewrite H5.
+        assert (G ~ U +~ map (length G +>) (G' ~ e1)
+                |-e length G +> (s0 *^ ` (length (G +~ G')))
+                : length G +> x).
+        { apply H. constructor. assumption. simpl. econstructor.
+          assumption. erewrite splice_sort. apply H. constructor. eassumption.
+          assumption. }
+      - simpl. apply hasType_inversion_lam in H0. do 2 destruct H0.
+        do 2 destruct H2. remember (length G +> T) as T'. econstructor.
+        econstructor. erewrite splice_sort. apply H. constructor.
+        eassumption. assumption. 
+        assert (tVar ` (length (G ~ U +~ map (length G +>) G'))
+                = length G +> ` (length (G +~ G'))).
+        { rewrite length_elim_middle. repeat rewrite app_length. 
+          rewrite map_length. simpl. 
+          replace (length G <=? length G' + length G) with true. reflexivity.
+          symmetry. apply Nat.leb_le. lia. }
+        rewrite H4. 
+        assert (G ~ U +~ map (length G +>) (G' ~ e1) 
+                |-e length G +> (e2 *^ ` (length (G +~ G'))) 
+                    : length G +> (x0 *^ ` (length (G +~ G')))).
+        { apply H. constructor. simpl. eassumption. simpl. econstructor.
+          assumption. erewrite splice_sort. apply H. constructor. eassumption.
+          assumption. }
+        assert (map (length G +>) G' ~ length G +> e1 
+                = map (length G +>) (G' ~ e1)) by reflexivity.
+        rewrite app_comm_cons. rewrite H6. repeat rewrite splice_open in H5.
+        exact H5. subst. 
+        replace (TAll (length G +> e1) (length G +> x0)) 
+          with (length G +> (TAll e1 x0)). apply eq_splice. apply e_sym.
+        assumption. reflexivity.
+      - simpl. apply hasType_inversion_app in H0. do 2 destruct H0. 
+        do 2 destruct H2. remember (length G +> T) as T'. econstructor.
+        econstructor. 
+        assert (G ~ U +~ map (length G +>) G' 
+                |-e length G +> e1 
+                : length G +> (TAll x0 x)).
+        { apply H. constructor. assumption. assumption. }
+        simpl in H4. exact H4. apply H. constructor. assumption. assumption.
+        rewrite <- splice_open. subst. apply eq_splice. apply e_sym.
+        assumption.
+      - simpl. apply hasType_inversion_sig in H0. do 2 destruct H0.
+        do 2 destruct H2. remember (length G +> T) as T'. 
+        apply t_conv with (T := length G +> x0). econstructor.
+        assert (forall s : sort, TSort s = length G +> s) by reflexivity.
+        rewrite H4. apply H. constructor. eassumption. assumption.
+        assert (tVar ` (length (G ~ U +~ map (length G +>) G')) = 
+                length G +> ` (length (G +~ G'))).
+        { rewrite length_elim_middle. simpl. 
+          replace (length G <=? length (G +~ G')) with true. 
+          repeat rewrite app_length. rewrite map_length. reflexivity. 
+          symmetry. rewrite Nat.leb_le. rewrite app_length. lia. }
+        rewrite H4. rewrite <- splice_open.
+        assert ((G ~ U +~ map (length G +>) G') ~ length G +> e1 = 
+                G ~ U +~ map (length G +>) (G' ~ e1)) by reflexivity.
+        rewrite H5. assert (forall s, TSort s = length G +> s) by reflexivity.
+        rewrite H6. apply H. constructor. apply H3. simpl. econstructor.
+        assumption. rewrite H6. apply H. constructor. eassumption. assumption.
+        subst. apply eq_splice. apply e_sym. assumption.
+      - simpl. apply hasType_inversion_pair in H0. destruct H0. 
+        do 2 destruct H2. do 2 destruct H3. destruct H4. destruct H5. subst.
+        remember (length G +> T) as T'. simpl. econstructor. econstructor.
+        econstructor. erewrite splice_sort. apply H. 
+      - admit.
+      - admit.
+    
+
+        
+        
 
   (*************************************************************************
    * Embedding of System D<:> 
@@ -889,42 +974,6 @@ Module CC.
     (T & 
       ((tId T) & (tId T) :[TSig (TAll T T) (TAll T T)])
     :[TSig prop (TSig (TAll #0 #1) (TAll #1 #2))]).
-
-  Definition wfTy G T := hasType G T prop.
-  Notation "G |-* T" := (wfTy G T) (at level 90) : cc_scope.
-
-  (* Type formation: Our shallow embedding lives in prop, so well formed types
-     are simply types that live in prop. *)
-  Lemma wf_bot : forall G, G |-cc -> G |-* TBot.
-  Proof.
-    repeat (constructor || assumption || econstructor).
-  Qed.
-
-  Lemma wf_top : forall G, G |-cc -> G |-* TTop.
-  Proof.
-    repeat (constructor || assumption || econstructor).
-  Qed.
-
-  Lemma wf_all : forall G T U,
-    G |-* T ->
-    G ~ T |-* U *^ varF (length G) ->
-    G |-* TAll T U.
-  Proof.
-    repeat (constructor || assumption || eassumption || econstructor).
-  Qed.
-
-  Lemma wf_typ : forall G T U,
-    G |-* T ->
-    G |-* U ->
-    G |-* TTyp T U.
-  Proof.
-    intros.
-    assert (T *^ varF (length G) = T). admit (* TODO: From G |-* T *).
-    assert (G ~ TSort prop |-* T). admit (* TODO: Weakening on H *).
-    assert (forall i t, e{i :-> t} U = U). admit (* TODO: From G |-* T *).
-    assert (forall T1 T2, G ~ TSort prop ~ T1 ~ T2 |-* U). 
-    admit (* TODO: Weakening on H0. *).
-    assert (G ~ TSort prop |-* TAll T (varF (length G))).
     { econstructor. eauto. simpl. repeat constructor. econstructor; eauto. }
     econstructor.
     - constructor. eauto.
@@ -1017,6 +1066,8 @@ End CC.
 
 (***************************************************************************
  * Translation
+ * -----------
+ * [ ] Presyntax
  * -----------
  * [ ] Presyntax
  * [ ] Types
